Demo.v
@@ -2,6 +2,7 @@ Require Export MQFair.
 Require Export MQUM.
 Require Export MQMM.
 Require Export Bound.
+Require Export Uniqueness.
 (*This is a demo file and it contains results from our paper titled
 "Verified Double Sided Auctions in Financial Markets". This file contains
 three important processes and their main theorems of corrctness. Besides we also have a combinatorial property.
@@ -24,6 +25,14 @@ M is a matching in the list of bids B and list of asks A.
 8. 
 *)
 
+Section Demo.
+
+
+
+
+Hypothesis unique_timestampbid:forall b1 b2, (btime b1 = btime b2) -> b1 = b2.
+Hypothesis unique_timestampask:forall s1 s2, (stime s1 = stime s2) -> s1 = s2.
+
 (*############### 1. FAIR  #######################*)
 
 (*This is FAIR process. The FAIR process takes a matching M and a lis of duplicate-free Bids B and a list of duplicate-free Asks A as inputs. 
@@ -31,16 +40,16 @@ It outputs a fair matching on the same list of bids and asks (B and A)
 without compromizing on the total volume of M. A direct cosequence of this
  result is that there always exists a maximum matching which is also fair.*)
 
+(*
 Definition fair_on_asks (M: list fill_type) (A: list Ask):=
-  (forall s s', In s A /\ In s' A -> s < s' -> In s' (asks_of M) ->
+  (forall s s', In s A /\ In s' A -> s <> s' -> by_sp s s' -> In s' (asks_of M) ->
   (ttqa M s')>0 -> 
   (In s (asks_of M)/\(ttqa M s= sq s))).
 
 Definition fair_on_bids (M: list fill_type)(B: list Bid):=
-  (forall b b', In b B /\ In b' B -> b > b' -> In b' (bids_of M) -> 
+  (forall b b', In b B /\ In b' B -> b <> b' -> by_dbp b b' -> In b' (bids_of M) -> 
   (ttqb M b')>0-> 
   (In b (bids_of M)/\(ttqb M b= bq b))).
- 
 
 Definition Is_fair (M: list fill_type) (B: list Bid) (A: list Ask) 
   :=  fair_on_asks M A /\ fair_on_bids M B.
@@ -48,16 +57,13 @@ Definition Is_fair (M: list fill_type) (B: list Bid) (A: list Ask)
 Definition FAIR (M: list fill_type) (B: list Bid) (A: list Ask) :=
 FOB (sort m_dbp (FOA (sort m_sp M) (sort by_sp A))) (sort by_dbp B).
 
-
-Theorem FAIR_main (M: list fill_type)(B: list Bid)(A:list Ask)
-(NDB: NoDup B) (NDA: NoDup A)(NZT:(forall m, In m M -> (tq m) > 0))
-(NZA:(forall a0, In a0 A -> (sq a0) > 0))
-(Hanti: (antisymmetric by_sp)/\(antisymmetric by_dbp) ): 
-matching_in B A M-> 
-(matching_in B A (FAIR M B A))/\
-(Is_fair (FAIR M B A) B A)/\
-(QM(M)= QM((FAIR M B A))).
-Proof. apply FAIR_correct. all: auto. Qed.
+*)
+Theorem FAIR_main (M: list fill_type)(B: list Bid)(A:list Ask)(NDB: NoDup B)
+        (NDA: NoDup A)(NZT:(forall m, In m M -> (tq m) > 0))
+         (NZA:(forall a0, In a0 A -> (sq a0) > 0)): 
+        matching_in B A M-> 
+        (matching_in B A (FAIR M B A))/\(Is_fair (FAIR M B A) B A)/\(QM(M)= QM((FAIR M B A))).
+Proof. eapply FAIR_correct with (M:=M)(B:=B)(A:=A). all: auto. Qed.
 
 (*############### 2. UM  #######################*)
 
@@ -67,12 +73,12 @@ of UM is fair, uniform, IR and maximum amongst all the uniform matchings.
 This process is used by the financial exchanges (stock, commodities etc. )
 to match buyers and sellers.*)
 
-
+(*
 Definition UM B A:=  
 replace_column 
 (UM_aux (sort by_dbp B) (sort by_sp A) 0 0) 
 (uniform_price (sort by_dbp B) (sort by_sp A)).
-
+*)
 
 Theorem UM_main (B:list Bid)(A:list Ask)(M:list fill_type)
 (NZT: forall m : fill_type, In m M -> tq m > 0)
@@ -96,10 +102,10 @@ It outputs a matching on the same list of bids and asks (B and A). The output
 of MM is fair, IR and maximum amongst all the matchings on B and A.
 *)
 
-
+(*
 Definition MM B A:=  
 (MM_aux (sort by_dbp B) (sort by_dsp A) 0 0).
-
+*)
 
 Theorem MM_main (B:list Bid)(A:list Ask)(M:list fill_type)
 (NZB: forall b, In b B -> (bq b)>0)
@@ -148,9 +154,35 @@ QM(M)<= QB(buyers_above p B) + QA(sellers_below p A).
 Proof. apply bound_on_M. all:auto. Qed.
 
 
+(*Below we have our main uniqueness results from the paper.*)
+
+
+Theorem uniqueness (M1 M2: list fill_type) (B:list Bid) (A:list Ask)
+(NZB: forall b, In b B -> (bq b)>0)
+(NZA: forall a, In a A -> (sq a)>0)
+(NDB: NoDup B)(NDA: NoDup A)
+(b:Bid) (a:Ask):
+(matching_in B A M1)/\ (matching_in B A M2) /\(QM(M1) = QM(M2))
+/\(Is_fair M1 B A) /\ (Is_fair M2 B A)
+-> (ttqa M1 a = ttqa M2 a)/\(ttqb M1 b = ttqb M2 b).
+Proof. apply completeness. all:auto. Qed. 
+
+
+
+Theorem reverse_uniqueness (M1 M2: list fill_type) (B:list Bid) (A:list Ask)
+(NZB: forall b, In b B -> (bq b)>0)
+(NZA: forall a, In a A -> (sq a)>0)
+(NDB: NoDup B)(NDA: NoDup A):
+(matching_in B A M1)-> (matching_in B A M2) ->
+(forall b, (ttqb M1 b = ttqb M2 b))/\(forall a, (ttqa M1 a = ttqa M2 a))
+->(Is_fair M1 B A)  
+-> (Is_fair M2 B A).
+Proof. apply soundness. all:auto. Qed.
+
+
 (*Note: For all other intermediate results please look at respective files*)
 
-
+End Demo.
 
 (*################ Extracted Programs ############################*)
 (*Now we extract programs from the above process*)
@@ -161,7 +193,23 @@ Recursive Extraction FAIR.
 Recursive Extraction UM.
 Recursive Extraction MM_FAIR.
 
+(*This part is tellling coq to extract nat, bool, additions, multiplications, equality and less than
+ Into the corrsponding OCaml types. *)
+Require Import ExtrOcamlBasic.
+Require Import ExtrOcamlString.
+Extract Inductive bool => "bool" [ "true" "false" ].
+Extract Inductive nat => "int"
+  [ "0" "(fun x -> x + 1)" ]
+  "(fun zero succ n -> if n=0 then zero () else succ (n-1))".
+Extract Constant plus => "( + )".
+Extract Constant mult => "( * )".
+Extract Constant Nat.eqb => "( = )".
+Extract Constant Nat.leb => "(<=)".
+
 Extraction  Language OCaml.
+Extraction "Demonstration/certified.ml" ttqa ttqb UM MM FAIR.
+(*
 Recursive Extraction FAIR.
 Recursive Extraction UM.
 Recursive Extraction MM_FAIR.
+*)
