Uniqueness.v
@@ -1,0 +1,508 @@
+Require Import ssreflect ssrbool.
+Require Export Lists.List.
+Require Export GenReflect SetSpecs.
+Require Export DecList.
+Require Export DecSort.
+Require Export mBidAsk.
+Require Export Quantity.
+Require Export mMatching.
+Require Export MatchingAlter.
+Require Export MQFair.
+
+
+Section Uniqueness.
+
+(*
+Definition Optimal_IR_Uniform (M:list fill_type)(B:list Bid)(A:list Ask): 
+matching_in B A M/\ Is_IR M /\ Uniform M/\(forall M', (matching_in B A M'/\Is_IR M' /\ Uniform M') -> QM(M')<=QM(M)).
+*)
+Lemma less_Q_implies_less_qa (M1 M2: list fill_type)(A:list Ask):
+QMa M1 A < QMa M2 A ->
+exists a' : Ask, (In a' A)/\(ttqa M1 a' < ttqa M2 a').
+Proof. revert M1 M2. induction A. intros. simpl in H.
+lia. intros. simpl in H. 
+assert(Ha:(ttqa M1 a < ttqa M2 a)\/(ttqa M1 a >= ttqa M2 a)).
+lia. destruct Ha. exists a. auto. assert(QMa M1 A < QMa M2 A).
+lia. apply IHA in H1. destruct H1. destruct H1. exists x. auto. Qed.
+
+Lemma size_equal_and_gt_imply_lt_ask (M1 M2: list fill_type)(A:list Ask)
+(a:Ask):
+(QMa M1 A = QMa M2 A) -> In a A -> (ttqa M1 a > ttqa M2 a) -> 
+(exists a', (In a' A)/\(ttqa M1 a' < ttqa M2 a')).
+
+Proof. intros. 
+       induction A. elim H0. 
+       simpl in H0. destruct H0. subst a0.
+       simpl in H. assert(HM:QMa M1 A < QMa M2 A).
+       lia. apply less_Q_implies_less_qa with (A:=A) in HM.
+       destruct HM. destruct H0. exists x. auto.
+       simpl in H.
+       assert(Ha:(ttqa M1 a0 < ttqa M2 a0)
+       \/(ttqa M1 a0 = ttqa M2 a0)
+       \/(ttqa M1 a0 > ttqa M2 a0)).
+       lia.
+       destruct Ha.
+       exists a0. auto.
+       destruct H2.
+       assert(QMa M1 A = QMa M2 A).
+       lia. apply IHA in H3.
+       destruct H3. destruct H3. exists x. auto.
+       auto.
+       assert(QMa M1 A < QMa M2 A). lia.
+       apply less_Q_implies_less_qa with (A:=A) in H3.
+       destruct H3. destruct H3. exists x. auto. Qed.
+        
+
+
+
+Lemma Qsize_equal_and_gt_imply_lt_ask (M1 M2: list fill_type)(A:list Ask)
+(NDA: NoDup A)(a:Ask):
+(QM(M1) = QM(M2)) -> (ttqa M1 a > ttqa M2 a) -> asks_of M1 [<=] A
+-> asks_of M2 [<=] A ->
+(exists a', (In a' A)/\(ttqa M1 a' < ttqa M2 a')).
+Proof. intros. apply QM_equal_QMa in H1 as H3. apply QM_equal_QMa in H2 as H4.
+       rewrite <- H3 in H. rewrite <- H4 in H.
+       assert(Ha1:In a (asks_of M1)). apply ttqa_intro1. lia.
+       assert (Ha2: In a A). eauto.
+       apply size_equal_and_gt_imply_lt_ask with (a:=a). all:auto. Qed. 
+       
+
+
+Theorem completeness_asks (M1 M2: list fill_type) (B:list Bid) (A:list Ask)
+(NZB: forall b, In b B -> (bq b)>0)
+(NZA: forall a, In a A -> (sq a)>0)
+(NDA: NoDup A)(a:Ask):
+  (matching_in B A M1)/\ (matching_in B A M2) 
+  /\(QM(M1) = QM(M2))
+  /\(fair_on_asks M1 A) /\ (fair_on_asks M2 A)
+    -> (ttqa M1 a = ttqa M2 a).
+Proof. intros. destruct H. destruct H0. destruct H1. destruct H2. 
+unfold fair_on_asks in H2. unfold fair_on_asks in H3.
+assert(Hta:ttqa M1 a = ttqa M2 a\/ttqa M1 a <> ttqa M2 a).
+eauto. destruct Hta. auto.
+assert(Hga:ttqa M1 a > ttqa M2 a\/ttqa M1 a < ttqa M2 a).
+ lia. destruct Hga. 
+  (*Case when there exists an ask a such that it's total trade quantities is more in M1 than M2*)
+  { assert(exists a', (In a' A)/\(ttqa M1 a' < ttqa M2 a')).
+    {  
+      apply Qsize_equal_and_gt_imply_lt_ask with (a:=a). all:auto.
+      apply H. apply H0.
+    }
+    destruct H6 as [a' H6]. destruct H6.
+    assert(Ha: (by_sp a a')\/(by_sp a' a)). apply by_sp_P.
+    destruct Ha. 
+    (*Case when a is more competitive ask than a' *)
+    { assert(ttqa M2 a = 0\/ttqa M2 a <>0) by eauto.
+      destruct H9.  (*Case when more competitive does not belongs to M2*)
+        { destruct (a_eqb a a') eqn:Haa'. move /eqP in Haa'. subst. lia.
+          assert(HqaM1: ttqa M1 a>0). lia. assert(HM1A:In a (asks_of M1)). 
+          { apply ttqa_intro1. lia. }
+          assert(HA:In a A). apply H in  HM1A. auto. 
+          assert(HqaM2: ttqa M2 a'>0). lia. assert(HM2A:In a' (asks_of M2)). 
+          { apply ttqa_intro1. lia. }
+          assert(HA2:In a' A). apply H0 in  HM2A. auto.
+          apply H3 in H8. destruct H8. specialize (NZA a). 
+          apply NZA in  HA. lia. auto. move /eqP in Haa'.  auto. 
+          auto. lia. 
+        } (*Case when more competitive belongs to M2*)
+        { assert(ttqa M1 a = 0\/ttqa M1 a <>0) by eauto.
+          destruct H10.
+          { lia. }
+          { destruct (a_eqb a a') eqn:Haa'. move /eqP in Haa'. subst. lia.
+            assert(HqaM1: ttqa M1 a>0). lia. assert(HM1A:In a (asks_of M1)). 
+            { apply ttqa_intro1. lia. }
+            assert(HA:In a A). apply H in  HM1A. auto. 
+            assert(HqaM2: ttqa M2 a'>0). lia. assert(HM2A:In a' (asks_of M2)). 
+            { apply ttqa_intro1. lia. }
+            assert(HA2:In a' A). apply H0 in  HM2A. auto.
+            assert(ttqa M2 a' >0) by lia. 
+            apply H3 with (s:=a)(s':=a') in H11 as H13.
+            destruct H13. assert(ttqa M1 a <= sq a). apply H.
+            auto. lia. 
+            all:auto. move /eqP in Haa'. auto.
+          }
+        }
+      }
+    (*Case when a' is more competitive ask than a *)
+    { assert(ttqa M1 a' = 0\/ttqa M1 a' <>0) by eauto.
+      destruct H9.  (*Case when more competitive does not belongs to M1*)
+        { destruct (a_eqb a a') eqn:Haa'. move /eqP in Haa'. subst. lia.
+          assert(HqaM1: ttqa M2 a'>0). lia. assert(HM2A:In a' (asks_of M2)). 
+          { apply ttqa_intro1. lia. }
+          assert(HA:In a' A). apply H0 in HM2A. auto. 
+          assert(HqaM2: ttqa M1 a>0). lia. assert(HM1A:In a (asks_of M1)). 
+          { apply ttqa_intro1. lia. }
+          assert(HA2:In a A). apply H in  HM1A. auto.
+          apply H2 in H8. destruct H8. specialize (NZA a'). 
+          apply NZA in  HA. lia. auto. move /eqP in Haa'.  auto. 
+          auto. lia. 
+        } (*Case when more competitive belongs to M2*)
+        { assert(ttqa M2 a' = 0\/ttqa M2 a' <>0) by eauto.
+          destruct H10.
+          { lia. }
+          { destruct (a_eqb a a') eqn:Haa'. move /eqP in Haa'. subst. lia.
+            assert(HqaM1: ttqa M2 a'>0). lia. assert(HM2A:In a' (asks_of M2)). 
+            { apply ttqa_intro1. lia. }
+            assert(HA:In a' A). apply H0 in HM2A. auto. 
+            assert(HqaM2: ttqa M1 a>0). lia. assert(HM1A:In a (asks_of M1)). 
+            { apply ttqa_intro1. lia. }
+            assert(HA2:In a A). apply H in  HM1A. auto.
+            apply H2 with (s:=a')(s':=a) in H8 as H12. destruct H12.
+            assert(ttqa M2 a' <= sq a'). apply H0.
+            auto. lia. 
+            all:auto. move /eqP in Haa'. auto.
+          }
+        }
+      }
+    }
+      (*Case when there exists an ask a such that it's total trade quantities is more in M1 than M2*)
+  { assert(exists a', (In a' A)/\(ttqa M1 a' > ttqa M2 a')).
+    {  
+      apply Qsize_equal_and_gt_imply_lt_ask with (a:=a). all:auto.
+      apply H0. apply H.
+    }
+    destruct H6 as [a' H6]. destruct H6.
+    assert(Ha: (by_sp a a')\/(by_sp a' a)). apply by_sp_P.
+    destruct Ha. 
+    (*Case when a is more competitive ask than a' *)
+    { assert(ttqa M1 a = 0\/ttqa M1 a <>0) by eauto.
+      destruct H9.  (*Case when more competitive does not belongs to M2*)
+        { destruct (a_eqb a a') eqn:Haa'. move /eqP in Haa'. subst. lia.
+          assert(HqaM2: ttqa M2 a>0). lia. assert(HM2A:In a (asks_of M2)). 
+          { apply ttqa_intro1. lia. }
+          assert(HA:In a A). apply H0 in  HM2A. auto. 
+          assert(HqaM1: ttqa M1 a'>0). lia. assert(HM1A:In a' (asks_of M1)). 
+          { apply ttqa_intro1. lia. }
+          assert(HA2:In a' A). apply H0 in HM2A. auto.
+          eapply H2 with (s:=a) in HqaM1. destruct HqaM1. specialize (NZA a). 
+          apply NZA in  HA. lia. auto. move /eqP in Haa'.  auto. 
+          auto. auto. 
+        } (*Case when more competitive belongs to M2*)
+        { assert(ttqa M2 a = 0\/ttqa M2 a <>0) by eauto.
+          destruct H10.
+          { lia. }
+          { destruct (a_eqb a a') eqn:Haa'. move /eqP in Haa'. subst. lia.
+            assert(HqaM2: ttqa M2 a>0). lia. assert(HM2A:In a (asks_of M2)). 
+            { apply ttqa_intro1. lia. }
+            assert(HA:In a A). apply H0 in  HM2A. auto. 
+            assert(HqaM1: ttqa M1 a'>0). lia. assert(HM1A:In a' (asks_of M1)). 
+            { apply ttqa_intro1. lia. }
+            assert(HA2:In a' A). apply H0 in HM2A. auto.
+            apply H2 with (s:=a)(s':=a') in HqaM1 as H13.
+            destruct H13. assert(ttqa M2 a <= sq a). apply H0.
+            auto. lia. 
+            all:auto. move /eqP in Haa'. auto.
+          }
+        }
+      }
+    (*Case when a' is more competitive ask than a *)
+    { assert(ttqa M2 a' = 0\/ttqa M2 a' <>0) by eauto.
+      destruct H9.  (*Case when more competitive does not belongs to M1*)
+        { destruct (a_eqb a a') eqn:Haa'. move /eqP in Haa'. subst. lia.
+          assert(HqaM2: ttqa M2 a>0). lia. assert(HM2A:In a (asks_of M2)). 
+          { apply ttqa_intro1. lia. }
+          assert(HA:In a A). apply H0 in HM2A. auto. 
+          assert(HqaM1: ttqa M1 a'>0). lia. assert(HM1A:In a' (asks_of M1)). 
+          { apply ttqa_intro1. lia. }
+          assert(HA2:In a' A). apply H in  HM1A. auto.
+          apply H3 in H8. destruct H8. specialize (NZA a'). 
+          apply NZA in  HA2. lia. auto. move /eqP in Haa'.  auto. 
+          auto. lia. 
+        } (*Case when more competitive belongs to M2*)
+        { assert(ttqa M2 a = 0\/ttqa M2 a <>0) by eauto.
+          destruct H10.
+          { lia. }
+          { destruct (a_eqb a a') eqn:Haa'. move /eqP in Haa'. subst. lia.
+            assert(HqaM1: ttqa M2 a>0). lia. assert(HM2A:In a (asks_of M2)). 
+            { apply ttqa_intro1. lia. }
+            assert(HA:In a A). apply H0 in HM2A. auto. 
+            assert(HqaM2: ttqa M1 a'>0). lia. assert(HM1A:In a' (asks_of M1)). 
+            { apply ttqa_intro1. lia. }
+            assert(HA2:In a' A). apply H in  HM1A. auto.
+            apply H3 with (s:=a')(s':=a) in H8 as H12. destruct H12.
+            assert(ttqa M1 a' <= sq a'). apply H.
+            auto. lia. 
+            all:auto. move /eqP in Haa'. auto.
+          }
+        }
+      }
+    } Qed.
+
+
+
+
+Lemma less_Q_implies_less_qb (M1 M2: list fill_type)(B:list Bid):
+QMb M1 B < QMb M2 B ->
+exists b' : Bid, (In b' B)/\(ttqb M1 b' < ttqb M2 b').
+Proof. revert M1 M2. induction B as [|b B']. intros. simpl in H.
+lia. intros. simpl in H. 
+assert(Hb:(ttqb M1 b < ttqb M2 b)\/(ttqb M1 b >= ttqb M2 b)).
+lia. destruct Hb. exists b. auto. assert(QMb M1 B' < QMb M2 B').
+lia. apply IHB' in H1. destruct H1. destruct H1. exists x. auto. Qed.
+
+Lemma size_equal_and_gt_imply_lt_bid (M1 M2: list fill_type)(B:list Bid)
+(b:Bid):
+(QMb M1 B = QMb M2 B) -> In b B -> (ttqb M1 b > ttqb M2 b) -> 
+(exists b', (In b' B)/\(ttqb M1 b' < ttqb M2 b')).
+
+Proof. intros. 
+       induction B as [|b0 B']. elim H0. 
+       simpl in H0. destruct H0. subst b0.
+       simpl in H. assert(HM:QMb M1 B' < QMb M2 B').
+       lia. apply less_Q_implies_less_qb with (B:=B') in HM.
+       destruct HM. destruct H0. exists x. auto.
+       simpl in H.
+       assert(Hb:(ttqb M1 b0 < ttqb M2 b0)
+       \/(ttqb M1 b0 = ttqb M2 b0)
+       \/(ttqb M1 b0 > ttqb M2 b0)).
+       lia.
+       destruct Hb.
+       exists b0. auto.
+       destruct H2.
+       assert(QMb M1 B' = QMb M2 B').
+       lia. apply IHB' in H3.
+       destruct H3. destruct H3. exists x. auto.
+       auto.
+       assert(QMb M1 B' < QMb M2 B'). lia.
+       apply less_Q_implies_less_qb with (B:=B') in H3.
+       destruct H3. destruct H3. exists x. auto. Qed.
+        
+
+
+
+Lemma Qsize_equal_and_gt_imply_lt_bid (M1 M2: list fill_type)(B:list Bid)
+(NDB: NoDup B)(b:Bid):
+(QM(M1) = QM(M2)) -> (ttqb M1 b > ttqb M2 b) -> bids_of M1 [<=] B
+-> bids_of M2 [<=] B ->
+(exists b', (In b' B)/\(ttqb M1 b' < ttqb M2 b')).
+Proof. intros. apply QM_equal_QMb in H1 as H3. apply QM_equal_QMb in H2 as H4.
+       rewrite <- H3 in H. rewrite <- H4 in H.
+       assert(Hb1:In b (bids_of M1)). apply ttqb_intro1. lia.
+       assert (Hb2: In b B). eauto.
+       apply size_equal_and_gt_imply_lt_bid with (b:=b). all:auto. Qed. 
+       
+
+
+Theorem completeness_bids (M1 M2: list fill_type) (B:list Bid) (A:list Ask)
+(NZB: forall b, In b B -> (bq b)>0)
+(NZA: forall a, In a A -> (sq a)>0)
+(NDB: NoDup B)(b:Bid):
+  (matching_in B A M1)/\ (matching_in B A M2) 
+  /\(QM(M1) = QM(M2))
+  /\(fair_on_bids M1 B) /\ (fair_on_bids M2 B)
+    -> (ttqb M1 b = ttqb M2 b).
+Proof. intros. destruct H. destruct H0. destruct H1. destruct H2. 
+unfold fair_on_bids in H2. unfold fair_on_bids in H3.
+assert(Htb:ttqb M1 b = ttqb M2 b\/ttqb M1 b <> ttqb M2 b).
+eauto. destruct Htb. auto.
+assert(Hgb:ttqb M1 b > ttqb M2 b\/ttqb M1 b < ttqb M2 b).
+ lia. destruct Hgb. 
+  (*Case when there exists a bid a such that it's total trade quantities is more in M1 than M2*)
+  { assert(exists b', (In b' B)/\(ttqb M1 b' < ttqb M2 b')).
+    {  
+      apply Qsize_equal_and_gt_imply_lt_bid with (b:=b). all:auto.
+      apply H. apply H0.
+    }
+    destruct H6 as [b' H6]. destruct H6.
+    assert(Hb: (by_dbp b b')\/(by_dbp b' b)). apply by_dbp_P.
+    destruct Hb. 
+    (*Case when b is more competitive bid than b' *)
+    { assert(ttqb M2 b = 0\/ttqb M2 b <>0) by eauto.
+      destruct H9.  (*Case when more competitive does not belongs to M2*)
+        { destruct (b_eqb b b') eqn:Hbb'. move /eqP in Hbb'. subst. lia.
+          assert(HqbM1: ttqb M1 b>0). lia. assert(HM1B:In b (bids_of M1)). 
+          { apply ttqb_intro1. lia. }
+          assert(HB:In b B). apply H in  HM1B. auto. 
+          assert(HqbM2: ttqb M2 b'>0). lia. assert(HM2B:In b' (bids_of M2)). 
+          { apply ttqb_intro1. lia. }
+          assert(HB2:In b' B). apply H0 in  HM2B. auto.
+          apply H3 in H8. destruct H8. specialize (NZB b). 
+          apply NZB in HB. lia. auto. move /eqP in Hbb'.  auto. 
+          auto. lia. 
+        } (*Case when more competitive belongs to M2*)
+        { assert(ttqb M1 b = 0\/ttqb M1 b <>0) by eauto.
+          destruct H10.
+          { lia. }
+          { destruct (b_eqb b b') eqn:Hbb'. move /eqP in Hbb'. subst. lia.
+            assert(HqbM1: ttqb M1 b>0). lia. assert(HM1B:In b (bids_of M1)). 
+            { apply ttqb_intro1. lia. }
+            assert(HB:In b B). apply H in  HM1B. auto. 
+            assert(HqbM2: ttqb M2 b'>0). lia. assert(HM2B:In b' (bids_of M2)). 
+            { apply ttqb_intro1. lia. }
+            assert(HB2:In b' B). apply H0 in  HM2B. auto.
+            assert(ttqb M2 b' >0) by lia. 
+            apply H3 with (b:=b)(b':=b') in H11 as H13.
+            destruct H13. assert(ttqb M1 b <= bq b). apply H.
+            auto. lia. 
+            all:auto. move /eqP in Hbb'. auto.
+          }
+        }
+      }
+    (*Case when b' is more competitive bid than b *)
+    { assert(ttqb M1 b' = 0\/ttqb M1 b' <>0) by eauto.
+      destruct H9.  (*Case when more competitive does not belongs to M1*)
+        { destruct (b_eqb b b') eqn:Hbb'. move /eqP in Hbb'. subst. lia.
+          assert(HqbM1: ttqb M2 b'>0). lia. assert(HM2B:In b' (bids_of M2)). 
+          { apply ttqb_intro1. lia. }
+          assert(HB:In b' B). apply H0 in HM2B. auto. 
+          assert(HqbM2: ttqb M1 b>0). lia. assert(HM1B:In b (bids_of M1)). 
+          { apply ttqb_intro1. lia. }
+          assert(HB2:In b B). apply H in  HM1B. auto.
+          apply H2 in H8. destruct H8. specialize (NZB b'). 
+          apply NZB in  HB. lia. auto. move /eqP in Hbb'.  auto. 
+          auto. lia. 
+        } (*Case when more competitive belongs to M2*)
+        { assert(ttqb M2 b' = 0\/ttqb M2 b' <>0) by eauto.
+          destruct H10.
+          { lia. }
+          { destruct (b_eqb b b') eqn:Hbb'. move /eqP in Hbb'. subst. lia.
+            assert(HqbM1: ttqb M2 b'>0). lia. assert(HM2B:In b' (bids_of M2)). 
+            { apply ttqb_intro1. lia. }
+            assert(HB:In b' B). apply H0 in HM2B. auto. 
+            assert(HqbM2: ttqb M1 b>0). lia. assert(HM1B:In b (bids_of M1)). 
+            { apply ttqb_intro1. lia. }
+            assert(HB2:In b B). apply H in  HM1B. auto.
+            apply H2 with (b:=b')(b':=b) in H8 as H12. destruct H12.
+            assert(ttqb M2 b' <= bq b'). apply H0.
+            auto. lia. 
+            all:auto. move /eqP in Hbb'. auto.
+          }
+        }
+      }
+    }
+      (*Case when there exists an ask a such that it's total trade quantities is more in M1 than M2*)
+  { assert(exists b', (In b' B)/\(ttqb M1 b' > ttqb M2 b')).
+    {  
+      apply Qsize_equal_and_gt_imply_lt_bid with (b:=b). all:auto.
+      apply H0. apply H.
+    }
+    destruct H6 as [b' H6]. destruct H6.
+    assert(Hb: (by_dbp b b')\/(by_dbp b' b)). apply by_dbp_P.
+    destruct Hb. 
+    (*Case when b is more competitive bid than b' *)
+    { assert(ttqb M1 b = 0\/ttqb M1 b <>0) by eauto.
+      destruct H9.  (*Case when more competitive does not belongs to M2*)
+        { destruct (b_eqb b b') eqn:Hbb'. move /eqP in Hbb'. subst. lia.
+          assert(HqbM2: ttqb M2 b>0). lia. assert(HM2B:In b (bids_of M2)). 
+          { apply ttqb_intro1. lia. }
+          assert(HB:In b B). apply H0 in  HM2B. auto. 
+          assert(HqbM1: ttqb M1 b'>0). lia. assert(HM1B:In b' (bids_of M1)). 
+          { apply ttqb_intro1. lia. }
+          assert(HB2:In b' B). apply H0 in HM2B. auto.
+          eapply H2 with (b:=b) in HqbM1. destruct HqbM1. specialize (NZB b). 
+          apply NZB in  HB. lia. auto. move /eqP in Hbb'.  auto. 
+          auto. auto. 
+        } (*Case when more competitive belongs to M2*)
+        { assert(ttqb M2 b = 0\/ttqb M2 b <>0) by eauto.
+          destruct H10.
+          { lia. }
+          { destruct (b_eqb b b') eqn:Hbb'. move /eqP in Hbb'. subst. lia.
+            assert(HqbM2: ttqb M2 b>0). lia. assert(HM2B:In b (bids_of M2)). 
+            { apply ttqb_intro1. lia. }
+            assert(HB:In b B). apply H0 in  HM2B. auto. 
+            assert(HqbM1: ttqb M1 b'>0). lia. assert(HM1B:In b' (bids_of M1)). 
+            { apply ttqb_intro1. lia. }
+            assert(HB2:In b' B). apply H0 in HM2B. auto.
+            apply H2 with (b:=b)(b':=b') in HqbM1 as H13.
+            destruct H13. assert(ttqb M2 b <= bq b). apply H0.
+            auto. lia. 
+            all:auto. move /eqP in Hbb'. auto.
+          }
+        }
+      }
+    (*Case when b' is more competitive bid than b *)
+    { assert(ttqb M2 b' = 0\/ttqb M2 b' <>0) by eauto.
+      destruct H9.  (*Case when more competitive does not belongs to M1*)
+        { destruct (b_eqb b b') eqn:Hbb'. move /eqP in Hbb'. subst. lia.
+          assert(HqbM2: ttqb M2 b>0). lia. assert(HM2B:In b (bids_of M2)). 
+          { apply ttqb_intro1. lia. }
+          assert(HB:In b B). apply H0 in HM2B. auto. 
+          assert(HqbM1: ttqb M1 b'>0). lia. assert(HM1B:In b' (bids_of M1)). 
+          { apply ttqb_intro1. lia. }
+          assert(HB2:In b' B). apply H in  HM1B. auto.
+          apply H3 in H8. destruct H8. specialize (NZB b'). 
+          apply NZB in  HB2. lia. auto. move /eqP in Hbb'.  auto. 
+          auto. lia. 
+        } (*Case when more competitive belongs to M2*)
+        { assert(ttqb M2 b = 0\/ttqb M2 b <>0) by eauto.
+          destruct H10.
+          { lia. }
+          { destruct (b_eqb b b') eqn:Hbb'. move /eqP in Hbb'. subst. lia.
+            assert(HqbM1: ttqb M2 b>0). lia. assert(HM2B:In b (bids_of M2)). 
+            { apply ttqb_intro1. lia. }
+            assert(HB:In b B). apply H0 in HM2B. auto. 
+            assert(HqbM2: ttqb M1 b'>0). lia. assert(HM1B:In b' (bids_of M1)). 
+            { apply ttqb_intro1. lia. }
+            assert(HB2:In b' B). apply H in  HM1B. auto.
+            apply H3 with (b:=b')(b':=b) in H8 as H12. destruct H12.
+            assert(ttqb M1 b' <= bq b'). apply H.
+            auto. lia. 
+            all:auto. move /eqP in Hbb'. auto.
+          }
+        }
+      }
+    } Qed.
+
+
+Theorem completeness (M1 M2: list fill_type) (B:list Bid) (A:list Ask)
+(NZB: forall b, In b B -> (bq b)>0)
+(NZA: forall a, In a A -> (sq a)>0)
+(NDB: NoDup B)(NDA: NoDup A)
+(b:Bid) (a:Ask):
+(matching_in B A M1)/\ (matching_in B A M2) /\(QM(M1) = QM(M2))
+/\(Is_fair M1 B A) /\ (Is_fair M2 B A)
+-> (ttqa M1 a = ttqa M2 a)/\(ttqb M1 b = ttqb M2 b).
+Proof. intros. split.
+                { apply completeness_asks with (B:=B)(A:=A). all:auto. 
+                  split. apply H. split. apply H. split. apply H. split. apply H. apply H.
+                }
+                { apply completeness_bids with (B:=B)(A:=A). all:auto. 
+                  split. apply H. split. apply H. split. apply H. split. apply H. apply H.
+                } Qed.
+
+
+
+Lemma soundness_asks (M1 M2: list fill_type) (B:list Bid) (A:list Ask)
+(NZB: forall b, In b B -> (bq b)>0)
+(NZA: forall a, In a A -> (sq a)>0)
+(NDA: NoDup A):
+(matching_in B A M1)-> (matching_in B A M2) ->(forall a, (ttqa M1 a = ttqa M2 a))
+->(fair_on_asks M1 A)  
+-> (fair_on_asks M2 A).
+Proof. unfold fair_on_asks. intros. specialize (H1 s') as Hs'.  specialize (H1 s) as Hs. 
+                  assert(ttqa M1 s' > 0). lia. 
+                  eapply H2 with (s:=s)(s':=s') in H8. destruct H8. 
+                  assert(In s A). apply H. auto. assert(In s' A). apply H0. auto. 
+                  specialize (NZA s). apply NZA in H10. assert(ttqa M2 s = sq s). lia. split.
+                  eapply ttqa_intro1.  lia. all: auto. apply ttqa_intro1. lia. Qed.
+
+Lemma soundness_bids (M1 M2: list fill_type) (B:list Bid) (A:list Ask)
+(NZB: forall b, In b B -> (bq b)>0)
+(NZA: forall a, In a A -> (sq a)>0)
+(NDA: NoDup B):
+(matching_in B A M1)-> (matching_in B A M2) ->(forall b, (ttqb M1 b = ttqb M2 b))
+->(fair_on_bids M1 B)  
+-> (fair_on_bids M2 B).
+Proof. unfold fair_on_bids. intros. specialize (H1 b') as Hb'.  specialize (H1 b) as Hb. 
+                  assert(ttqb M1 b' > 0). lia. 
+                  eapply H2 with (b:=b)(b':=b') in H7. destruct H7. 
+                  assert(In b B). apply H. auto. assert(In b' B). apply H0. auto. 
+                  specialize (NZB b). apply NZB in H9. assert(ttqb M2 b = bq b). lia. split.
+                  eapply ttqb_intro1.  lia. all: auto. apply ttqb_intro1. lia. Qed.
+
+
+Theorem soundness (M1 M2: list fill_type) (B:list Bid) (A:list Ask)
+(NZB: forall b, In b B -> (bq b)>0)
+(NZA: forall a, In a A -> (sq a)>0)
+(NDB: NoDup B)(NDA: NoDup A):
+(matching_in B A M1)-> (matching_in B A M2) ->
+(forall b, (ttqb M1 b = ttqb M2 b))/\(forall a, (ttqa M1 a = ttqa M2 a))
+->(Is_fair M1 B A)  
+-> (Is_fair M2 B A).
+Proof. intros. destruct H2. split.
+                { apply soundness_asks with (B:=B)(A:=A)(M2:=M2) in H2. all:auto. apply H1. 
+                }
+                { apply soundness_bids with (B:=B)(A:=A)(M2:=M2) in H3. all:auto. apply H1. 
+                } Qed.
+
+End Uniqueness.
